rewrite adaptation to use new function representation

Coq/loo_def.v
@@ -1024,3 +1024,25 @@ Hint Resolve (@empty_rename stmt).
 
 Hint Rewrite empty_rename.
 Hint Resolve empty_rename.
+
+Inductive in_ref : var -> ref -> Prop :=
+| in_r_var : forall x, in_ref x (r_var x)
+| in_r_fld : forall x f, in_ref x (r_fld x f).
+
+Inductive in_stmt : var -> stmt -> Prop :=
+| in_asgn_1 : forall x y z, in_ref x y ->
+                       in_stmt x (s_asgn y z)
+| in_asgn_2 : forall x y z, in_ref x z ->
+                       in_stmt x (s_asgn y z)
+| in_meth_1 : forall x y m ps, in_stmt x (s_meth x y m ps)
+| in_meth_2 : forall x y m ps, in_stmt y (s_meth x y m ps)
+| in_meth_3 : forall x y z m ps, (exists x', ps x' = Some z) ->
+                            in_stmt z (s_meth x y m ps)
+| in_new_1 : forall x C ps, in_stmt x (s_new x C ps)
+| in_new_2 : forall x y C ps, (exists z, ps z = Some y) ->
+                         in_stmt y (s_new x C ps)
+| in_stmts_1 : forall x s1 s2, in_stmt x s1 ->
+                          in_stmt x (s_stmts s1 s2)
+| in_stmts_2 : forall x s1 s2, in_stmt x s2 ->
+                          in_stmt x (s_stmts s1 s2)
+| in_retrn : forall x, in_stmt x (s_rtrn x).
